MRiscX/AbstractSyntax/Registers.lean
@@ -1,0 +1,183 @@
+
+inductive RegisterNr where
+  | zero
+  | one
+  | two
+  | three
+  | four
+  | five
+  | six
+  | seven
+  | eight
+  | nine
+  | ten
+  | eleven
+  | twelve
+  | thirteen
+  | fourteen
+  | fifteen
+  | sixteen
+  | seventeen
+  | eighteen
+  | nineteen
+  | twenty
+  | twentyone
+  | twentytwo
+  | twentythree
+  | twentyfour
+  | twentyfive
+  | twentysix
+  | twentyseven
+  | twentyeight
+  | twentynine
+  | thirty
+  | thirtyone
+deriving DecidableEq
+
+namespace RegisterNr
+
+def ofNat? (n : Nat) : Option RegisterNr :=
+  match n with
+  | 0 => some RegisterNr.zero
+  | 1 => some RegisterNr.one
+  | 2 => some RegisterNr.two
+  | 3 => some RegisterNr.three
+  | 4 => some RegisterNr.four
+  | 5 => some RegisterNr.five
+  | 6 => some RegisterNr.six
+  | 7 => some RegisterNr.seven
+  | 8 => some RegisterNr.eight
+  | 9 => some RegisterNr.nine
+  | 10 => some RegisterNr.ten
+  | 11 => some RegisterNr.eleven
+  | 12 => some RegisterNr.twelve
+  | 13 => some RegisterNr.thirteen
+  | 14 => some RegisterNr.fourteen
+  | 15 => some RegisterNr.fifteen
+  | 16 => some RegisterNr.sixteen
+  | 17 => some RegisterNr.seventeen
+  | 18 => some RegisterNr.eighteen
+  | 19 => some RegisterNr.nineteen
+  | 20 => some RegisterNr.twenty
+  | 21 => some RegisterNr.twentyone
+  | 22 => some RegisterNr.twentytwo
+  | 23 => some RegisterNr.twentythree
+  | 24 => some RegisterNr.twentyfour
+  | 25 => some RegisterNr.twentyfive
+  | 26 => some RegisterNr.twentysix
+  | 27 => some RegisterNr.twentyseven
+  | 28 => some RegisterNr.twentyeight
+  | 29 => some RegisterNr.twentynine
+  | 30 => some RegisterNr.thirty
+  | 31 => some RegisterNr.thirtyone
+  | _ => none
+
+def ofNat! (n : Nat) (d : RegisterNr) : RegisterNr :=
+  match n with
+  | 0 => RegisterNr.zero
+  | 1 => RegisterNr.one
+  | 2 => RegisterNr.two
+  | 3 => RegisterNr.three
+  | 4 => RegisterNr.four
+  | 5 => RegisterNr.five
+  | 6 => RegisterNr.six
+  | 7 => RegisterNr.seven
+  | 8 => RegisterNr.eight
+  | 9 => RegisterNr.nine
+  | 10 => RegisterNr.ten
+  | 11 => RegisterNr.eleven
+  | 12 => RegisterNr.twelve
+  | 13 => RegisterNr.thirteen
+  | 14 => RegisterNr.fourteen
+  | 15 => RegisterNr.fifteen
+  | 16 => RegisterNr.sixteen
+  | 17 => RegisterNr.seventeen
+  | 18 => RegisterNr.eighteen
+  | 19 => RegisterNr.nineteen
+  | 20 => RegisterNr.twenty
+  | 21 => RegisterNr.twentyone
+  | 22 => RegisterNr.twentytwo
+  | 23 => RegisterNr.twentythree
+  | 24 => RegisterNr.twentyfour
+  | 25 => RegisterNr.twentyfive
+  | 26 => RegisterNr.twentysix
+  | 27 => RegisterNr.twentyseven
+  | 28 => RegisterNr.twentyeight
+  | 29 => RegisterNr.twentynine
+  | 30 => RegisterNr.thirty
+  | 31 => RegisterNr.thirtyone
+  | _ => d
+
+instance : ToString RegisterNr where
+  toString
+  | RegisterNr.zero => "0"
+  | RegisterNr.one => "1"
+  | RegisterNr.two => "2"
+  | RegisterNr.three => "3"
+  | RegisterNr.four => "4"
+  | RegisterNr.five => "5"
+  | RegisterNr.six => "6"
+  | RegisterNr.seven => "7"
+  | RegisterNr.eight => "8"
+  | RegisterNr.nine => "9"
+  | RegisterNr.ten => "10"
+  | RegisterNr.eleven => "11"
+  | RegisterNr.twelve => "12"
+  | RegisterNr.thirteen => "13"
+  | RegisterNr.fourteen => "14"
+  | RegisterNr.fifteen => "15"
+  | RegisterNr.sixteen => "16"
+  | RegisterNr.seventeen => "17"
+  | RegisterNr.eighteen => "18"
+  | RegisterNr.nineteen => "19"
+  | RegisterNr.twenty => "20"
+  | RegisterNr.twentyone => "21"
+  | RegisterNr.twentytwo => "22"
+  | RegisterNr.twentythree => "23"
+  | RegisterNr.twentyfour => "24"
+  | RegisterNr.twentyfive => "25"
+  | RegisterNr.twentysix => "26"
+  | RegisterNr.twentyseven => "27"
+  | RegisterNr.twentyeight => "28"
+  | RegisterNr.twentynine => "29"
+  | RegisterNr.thirty => "30"
+  | RegisterNr.thirtyone => "31"
+
+  def eq (r1 r2 : RegisterNr) := (r1 == r2)
+
+end RegisterNr
+
+instance: BEq RegisterNr where
+  beq r1 r2 := r1 == r2
+
+
+structure RegisterName where
+  nr : RegisterNr
+  name : String
+deriving DecidableEq
+
+namespace RegisterName
+
+  def beq (n₁ n₂ : RegisterName) := n₁ == n₂
+
+  def beq_regNr (n₁ n₂ : RegisterName) := n₁.nr  == n₂.nr
+
+end RegisterName
+
+instance: BEq RegisterName where
+  beq n1 n2 := RegisterName.beq n1 n2
+
+instance: LawfulBEq RegisterName where
+  rfl := by
+    intros r
+    unfold BEq.beq
+    unfold instBEqRegisterName
+    simp [RegisterName.beq]
+  eq_of_beq := by
+    intros a b h
+    unfold BEq.beq instBEqRegisterName RegisterName.beq at h
+    simp at h
+    rw [h]
+
+instance: ToString RegisterName where
+   toString n := n.name
